Renamed functions name

src/functional/BST.dfy
@@ -9,11 +9,11 @@ datatype BST<T> = Leaf | Node(left:BST<T>, data:T, right:BST<T>)
 
 /** Properties:
  *
- *  Lemma_BSTInsertSameElemsPlusInserted(tree, d)
+ *  Lemma_BSTInsertIntegrity(tree, d)
  *    ==> ensures BST_ToMultiset(tree) + multiset{d} == BST_ToMultiset(BST_Insert(tree, d))
  *
- *  Lemma_BSTInsertIsOrdered(tree, d)
- *    ==> ensures bst_is_ordered(BST_Insert(tree, d))
+ *  Lemma_BSTInsertOrdering(tree, d)
+ *    ==> ensures bst_ordered(BST_Insert(tree, d))
  *
  *  Lemma_BSTInsertUpperBound(tree, d, b)
  *    ==> ensures bst_upper_bound(BST_Insert(tree, d), b)
@@ -37,16 +37,16 @@ function method BST_Insert(tree:BST<T>, d:T) : (result:BST<T>)
 
 /** Properties:
  *
- *  Lemma_BSTSameElementsThanInOrder(tree)
+ *  Lemma_InOrderIntegrity(tree)
  *    ==> ensures List_ToMultiset(BST_InOrder(tree)) == BST_ToMultiset(tree)
  *
- *  Lemma_BSTInOrderOrdered(tree)
- *    ==> ensures list_is_ordered(BST_InOrder(tree))
+ *  Lemma_BSTInOrderOrdering(tree)
+ *    ==> ensures list_ordered(BST_InOrder(tree))
  *
- *  Lemma_BSTUpperBoundThenInOrderUpperBound(tree, d)
+ *  Lemma_BSTInOrderUpperBound(tree, d)
  *    ==> ensures list_upper_bound(BST_InOrder(tree), d)
  *
- *  Lemma_BSTLowerBoundThenInOrderLowerBound(tree, d)
+ *  Lemma_BSTInOrderLowerBound(tree, d)
  *    ==> ensures list_lower_bound(BST_InOrder(tree), d)
  *
  */
@@ -62,10 +62,10 @@ function method BST_InOrder(tree:BST<T>) : (result:List<T>)
 
 /** Properties:
  *
- *  Lemma_BSTLoadIsOrdered(list)
- *    ==> ensures bst_is_ordered(BST_Load(list))
+ *  Lemma_BSTLoadOrdering(list)
+ *    ==> ensures bst_ordered(BST_Load(list))
  *
- *  Lemma_BSTLoadTreeElemsSameThanList(list:List<T>)
+ *  Lemma_BSTLoadIntegrity(list:List<T>)
  *    ==> ensures List_ToMultiset(list) == BST_ToMultiset(BST_Load(list))
  *
  */
@@ -89,14 +89,14 @@ function method BST_ToMultiset(tree:BST<T>) : multiset<T>
 
 // ---------------------- Predicates ---------------------- //
 
-predicate bst_is_ordered(tree:BST<T>)
+predicate bst_ordered(tree:BST<T>)
   decreases tree
 {
   match tree {
     case Leaf => true
     case Node(left, x, right) =>
-      bst_is_ordered(left) &&
-      bst_is_ordered(right) &&
+      bst_ordered(left) &&
+      bst_ordered(right) &&
       bst_upper_bound(left, x) &&
       bst_lower_bound(right, x)
   }
@@ -122,7 +122,7 @@ predicate bst_upper_bound(tree:BST<T>, d:T)
 
 // ------------------------ Lemmas ------------------------ //
 
-lemma {:induction tree} Lemma_BSTInsertSameElemsPlusInserted(tree:BST<T>, d:T)
+lemma {:induction tree} Lemma_BSTInsertIntegrity(tree:BST<T>, d:T)
   ensures BST_ToMultiset(BST_Insert(tree, d)) == BST_ToMultiset(tree) + multiset{d}
   decreases tree
 {
@@ -155,7 +155,7 @@ lemma {:induction tree} Lemma_BSTInsertSameElemsPlusInserted(tree:BST<T>, d:T)
             BST_ToMultiset(Node(BST_Insert(left, d), x , right));
               { assert BST_ToMultiset(Node(BST_Insert(left, d), x , right)) == BST_ToMultiset(BST_Insert(left, d)) + multiset{x} + BST_ToMultiset(right); }
             BST_ToMultiset(BST_Insert(left, d)) + multiset{x} + BST_ToMultiset(right);
-              { Lemma_BSTInsertSameElemsPlusInserted(left, d); }
+              { Lemma_BSTInsertIntegrity(left, d); }
           }
         } else {
           calc == {
@@ -164,7 +164,7 @@ lemma {:induction tree} Lemma_BSTInsertSameElemsPlusInserted(tree:BST<T>, d:T)
             BST_ToMultiset(Node(left, x, BST_Insert(right, d)));
               { assert BST_ToMultiset(Node(BST_Insert(left, d), x , right)) == BST_ToMultiset(left) + multiset{x} + BST_ToMultiset(BST_Insert(right, d)); }
             BST_ToMultiset(left) + multiset{x} + BST_ToMultiset(BST_Insert(right, d));
-              { Lemma_BSTInsertSameElemsPlusInserted(right, d); }
+              { Lemma_BSTInsertIntegrity(right, d); }
           }
         } }
         BST_ToMultiset(tree) + multiset{d};
@@ -172,41 +172,41 @@ lemma {:induction tree} Lemma_BSTInsertSameElemsPlusInserted(tree:BST<T>, d:T)
   }
 }
 
-lemma {:induction tree} Lemma_BSTInsertIsOrdered(tree:BST<T>, d:T)
-  requires bst_is_ordered(tree)
-  ensures bst_is_ordered(BST_Insert(tree, d))
+lemma {:induction tree} Lemma_BSTInsertOrdering(tree:BST<T>, d:T)
+  requires bst_ordered(tree)
+  ensures bst_ordered(BST_Insert(tree, d))
   decreases tree
 {
   match tree {
     case Leaf =>
       calc == {
-        bst_is_ordered(BST_Insert(tree, d));
+        bst_ordered(BST_Insert(tree, d));
           { assert tree == Leaf; }
-        bst_is_ordered(BST_Insert(Leaf, d));
+        bst_ordered(BST_Insert(Leaf, d));
           { assert BST_Insert(Leaf, d) == Node(Leaf, d, Leaf); }
-        bst_is_ordered(Node(Leaf, d, Leaf));
+        bst_ordered(Node(Leaf, d, Leaf));
         true;
       }
     case Node(left, x, right) =>
       calc == {
-        bst_is_ordered(BST_Insert(tree, d));
+        bst_ordered(BST_Insert(tree, d));
           { assert tree == Node(left, x, right); }
-        bst_is_ordered(BST_Insert(Node(left, x, right), d));
+        bst_ordered(BST_Insert(Node(left, x, right), d));
         { if (d < x) {
           calc == {
-            bst_is_ordered(Node(BST_Insert(left, d), x, right));
+            bst_ordered(Node(BST_Insert(left, d), x, right));
               { Lemma_BSTInsertUpperBound(left, d, x); }
               { assert bst_upper_bound(BST_Insert(left, d), x); }
-              { Lemma_BSTInsertIsOrdered(left, d); }
-            bst_is_ordered(Node(Leaf, d, Leaf));
+              { Lemma_BSTInsertOrdering(left, d); }
+            bst_ordered(Node(Leaf, d, Leaf));
           }
         } else {
           calc == {
-            bst_is_ordered(Node(left, x, BST_Insert(right, d)));
+            bst_ordered(Node(left, x, BST_Insert(right, d)));
               { Lemma_BSTInsertLowerBound(right, d, x); }
               { assert bst_lower_bound(BST_Insert(right, d), x); }
-              { Lemma_BSTInsertIsOrdered(right, d); }
-            bst_is_ordered(Node(Leaf, d, Leaf));
+              { Lemma_BSTInsertOrdering(right, d); }
+            bst_ordered(Node(Leaf, d, Leaf));
           }
         } }
         true;
@@ -215,7 +215,7 @@ lemma {:induction tree} Lemma_BSTInsertIsOrdered(tree:BST<T>, d:T)
 }
 
 lemma {:induction tree} Lemma_BSTInsertUpperBound(tree:BST<T>, d:T, b:T)
-  requires bst_is_ordered(tree)
+  requires bst_ordered(tree)
   requires bst_upper_bound(tree, b)
   requires b > d
   ensures bst_upper_bound(BST_Insert(tree, d), b)
@@ -251,7 +251,7 @@ lemma {:induction tree} Lemma_BSTInsertUpperBound(tree:BST<T>, d:T, b:T)
 }
 
 lemma {:induction tree} Lemma_BSTInsertLowerBound(tree:BST<T>, d:T, b:T)
-  requires bst_is_ordered(tree)
+  requires bst_ordered(tree)
   requires bst_lower_bound(tree, b)
   requires b <= d
   ensures bst_lower_bound(BST_Insert(tree, d), b)
@@ -286,8 +286,8 @@ lemma {:induction tree} Lemma_BSTInsertLowerBound(tree:BST<T>, d:T, b:T)
   }
 }
 
-lemma {:induction tree} Lemma_BSTSameElementsThanInOrder(tree:BST<T>)
-  requires bst_is_ordered(tree)
+lemma {:induction tree} Lemma_InOrderIntegrity(tree:BST<T>)
+  requires bst_ordered(tree)
   ensures BST_ToMultiset(tree) == List_ToMultiset(BST_InOrder(tree))
   decreases tree
 {
@@ -313,7 +313,7 @@ lemma {:induction tree} Lemma_BSTSameElementsThanInOrder(tree:BST<T>)
         List_ToMultiset(BST_InOrder(Node(left, x, right)));
           { assert List_ToMultiset(BST_InOrder(Node(left, x, right))) == List_ToMultiset(List_Concat(BST_InOrder(left), Cons(x, BST_InOrder(right)))); }
         List_ToMultiset(List_Concat(BST_InOrder(left), Cons(x, BST_InOrder(right))));
-          { Lemma_ListConcatSameElems(BST_InOrder(left), Cons(x, BST_InOrder(right))); }
+          { Lemma_ListConcatIntegrity(BST_InOrder(left), Cons(x, BST_InOrder(right))); }
         List_ToMultiset(BST_InOrder(left)) + List_ToMultiset(Cons(x, BST_InOrder(right)));
           { assert List_ToMultiset(Cons(x, BST_InOrder(right))) == List_ToMultiset(Cons(x, List_Empty)) + List_ToMultiset(BST_InOrder(right)); }
         List_ToMultiset(BST_InOrder(left)) + List_ToMultiset(Cons(x, List_Empty)) + List_ToMultiset(BST_InOrder(right));
@@ -323,46 +323,46 @@ lemma {:induction tree} Lemma_BSTSameElementsThanInOrder(tree:BST<T>)
         List_ToMultiset(BST_InOrder(left)) + multiset{x} + multiset{} + List_ToMultiset(BST_InOrder(right));
           { assert multiset{x} + multiset{} == multiset{x}; }
         List_ToMultiset(BST_InOrder(left)) + multiset{x} + List_ToMultiset(BST_InOrder(right));
-          { Lemma_BSTSameElementsThanInOrder(left); }
-          { Lemma_BSTSameElementsThanInOrder(right); }
+          { Lemma_InOrderIntegrity(left); }
+          { Lemma_InOrderIntegrity(right); }
         BST_ToMultiset(tree);
       }
   }
 }
 
-lemma {:induction tree} Lemma_BSTInOrderOrdered(tree:BST<T>)
-  requires bst_is_ordered(tree)
-  ensures list_is_ordered(BST_InOrder(tree))
+lemma {:induction tree} Lemma_BSTInOrderOrdering(tree:BST<T>)
+  requires bst_ordered(tree)
+  ensures list_ordered(BST_InOrder(tree))
 {
   match tree {
     case Leaf =>
       calc == {
-        list_is_ordered(BST_InOrder(tree));
+        list_ordered(BST_InOrder(tree));
           { assert tree == Leaf; }
-        list_is_ordered(BST_InOrder(Leaf));
+        list_ordered(BST_InOrder(Leaf));
           { assert BST_InOrder(Leaf) == List_Empty; }
-        list_is_ordered(List_Empty);
+        list_ordered(List_Empty);
         true;
       }
     case Node(left, x, right) =>
       calc == {
-        list_is_ordered(BST_InOrder(tree));
+        list_ordered(BST_InOrder(tree));
           { assert tree == Node(left, x, right); }
-        list_is_ordered(BST_InOrder(Node(left, x, right)));
+        list_ordered(BST_InOrder(Node(left, x, right)));
           { assert BST_InOrder(Node(left, x, right)) ==  List_Concat(BST_InOrder(left), Cons(x, BST_InOrder(right))); }
-        list_is_ordered(List_Concat(BST_InOrder(left), Cons(x, BST_InOrder(right))));
+        list_ordered(List_Concat(BST_InOrder(left), Cons(x, BST_InOrder(right))));
           { assert bst_lower_bound(right, x); }
-          { Lemma_BSTLowerBoundThenInOrderLowerBound(right, x); }
+          { Lemma_BSTInOrderLowerBound(right, x); }
           { assert bst_upper_bound(left, x); }
-          { Lemma_BSTUpperBoundThenInOrderUpperBound(left, x); }
-          { Lemma_ListConcatSortedWithMiddleElement(BST_InOrder(left), x, BST_InOrder(right)); }
+          { Lemma_BSTInOrderUpperBound(left, x); }
+          { Lemma_ListConcatWithMidElemOrdering(BST_InOrder(left), x, BST_InOrder(right)); }
         true;
       }
   }
 }
 
-lemma {:induction tree} Lemma_BSTUpperBoundThenInOrderUpperBound(tree:BST<T>, d:T)
-  requires bst_is_ordered(tree)
+lemma {:induction tree} Lemma_BSTInOrderUpperBound(tree:BST<T>, d:T)
+  requires bst_ordered(tree)
   requires bst_upper_bound(tree, d)
   ensures list_upper_bound(BST_InOrder(tree), d)
 {
@@ -386,14 +386,14 @@ lemma {:induction tree} Lemma_BSTUpperBoundThenInOrderUpperBound(tree:BST<T>, d:
             { assert list_upper_bound(BST_InOrder(left), d); }
             { assert list_upper_bound(BST_InOrder(right), d); }
             { assert d >= x; }
-            { Lemma_IfElemUpperBoundOfTwoListsThenIsUpperBoundOfConcat(BST_InOrder(left), BST_InOrder(right), d, x); }
+            { Lemma_ListConcatUpperBound(BST_InOrder(left), BST_InOrder(right), d, x); }
           true;
         }
   }
 }
 
-lemma {:induction tree} Lemma_BSTLowerBoundThenInOrderLowerBound(tree:BST<T>, d:T)
-  requires bst_is_ordered(tree)
+lemma {:induction tree} Lemma_BSTInOrderLowerBound(tree:BST<T>, d:T)
+  requires bst_ordered(tree)
   requires bst_lower_bound(tree, d)
   ensures list_lower_bound(BST_InOrder(tree), d)
 {
@@ -417,41 +417,41 @@ lemma {:induction tree} Lemma_BSTLowerBoundThenInOrderLowerBound(tree:BST<T>, d:
             { assert list_lower_bound(BST_InOrder(left), d); }
             { assert list_lower_bound(BST_InOrder(right), d); }
             { assert d <= x; }
-            { Lemma_IfElemLowerBoundOfTwoListsThenIsLowerBoundOfConcat(BST_InOrder(left), BST_InOrder(right), d, x); }
+            { Lemma_ListConcatLowerBound(BST_InOrder(left), BST_InOrder(right), d, x); }
           true;
         }
   }
 }
 
-lemma {:induction list} Lemma_BSTLoadIsOrdered(list:List<T>)
-  ensures bst_is_ordered(BST_Load(list))
+lemma {:induction list} Lemma_BSTLoadOrdering(list:List<T>)
+  ensures bst_ordered(BST_Load(list))
   decreases list
 {
   match list {
     case List_Empty =>
       calc == {
-        bst_is_ordered(BST_Load(list));
+        bst_ordered(BST_Load(list));
           { assert list == List_Empty; }
-        bst_is_ordered(BST_Load(List_Empty));
+        bst_ordered(BST_Load(List_Empty));
           { assert BST_Load(List_Empty) == Leaf; }
-        bst_is_ordered(Leaf);
-          { assert bst_is_ordered(Leaf) == true; }
+        bst_ordered(Leaf);
+          { assert bst_ordered(Leaf) == true; }
         true;
       }
     case Cons(head, tail) =>
       calc == {
-        bst_is_ordered(BST_Load(list));
+        bst_ordered(BST_Load(list));
           { assert list == Cons(head, tail); }
-        bst_is_ordered(BST_Load(Cons(head, tail)));
+        bst_ordered(BST_Load(Cons(head, tail)));
           { assert BST_Load(Cons(head, tail)) == BST_Insert(BST_Load(tail), head); }
-        bst_is_ordered(BST_Insert(BST_Load(tail), head));
-          { Lemma_BSTInsertIsOrdered(BST_Load(tail), head); }
+        bst_ordered(BST_Insert(BST_Load(tail), head));
+          { Lemma_BSTInsertOrdering(BST_Load(tail), head); }
         true;
       }
   }
 }
 
-lemma {:induction list} Lemma_BSTLoadTreeElemsSameThanList(list:List<T>)
+lemma {:induction list} Lemma_BSTLoadIntegrity(list:List<T>)
   ensures BST_ToMultiset(BST_Load(list)) == List_ToMultiset(list)
   decreases list
 {
@@ -477,9 +477,9 @@ lemma {:induction list} Lemma_BSTLoadTreeElemsSameThanList(list:List<T>)
         BST_ToMultiset(BST_Load(Cons(head, tail)));
           { assert BST_Load(Cons(head, tail)) == BST_Insert(BST_Load(tail), head); }
         BST_ToMultiset(BST_Insert(BST_Load(tail), head));
-          { Lemma_BSTInsertSameElemsPlusInserted(BST_Load(tail), head); }
+          { Lemma_BSTInsertIntegrity(BST_Load(tail), head); }
         BST_ToMultiset(BST_Load(tail)) + multiset{head};
-          { Lemma_BSTLoadTreeElemsSameThanList(tail); }
+          { Lemma_BSTLoadIntegrity(tail); }
         List_ToMultiset(list);
       }
   }
