src/imperative/TreeSort.dfy
@@ -3,22 +3,22 @@ include "../functional/BST.dfy"
 include "../functional/List.dfy"
 
 method TreeSort(L:List<int>) returns (sortedList:List<int>)
-  ensures list_is_ordered(sortedList)
+  ensures list_ordered(sortedList)
 {
   var tree: BST<int> := Leaf;
   var list := L;
 
   while list != List_Empty
-    invariant bst_is_ordered(tree)
+    invariant bst_ordered(tree)
     decreases list
   {
     var elem := List_Head(list);
-    Lemma_BSTInsertIsOrdered(tree, elem);
+    Lemma_BSTInsertOrdering(tree, elem);
     tree := BST_Insert(tree, elem);
     list := List_Tail(list);
   }
 
-  Lemma_BSTInOrderOrdered(tree);
+  Lemma_BSTInOrderOrdering(tree);
   sortedList := BST_InOrder(tree);
 
   return sortedList;
